Factor out Jrnl model

src/Dafny/jrnl/jrnl.s.dfy
@@ -7,133 +7,96 @@ include "kinds.s.dfy"
 Spec for sequential journal API, assuming we're using 2PL.
 */
 
-module JrnlSpec
+module {:extern "jrnl"} JrnlSpec
 {
 
-import opened Machine
-import opened Kinds
-import opened ByteSlice
-import opened Collections
+    import opened Machine
+    import opened Kinds
+    import opened ByteSlice
+    import opened Collections
 
-type Blkno = nat
-datatype Addr = Addr(blkno: Blkno, off: nat)
-type Object = seq<byte>
+    type Blkno = nat
+    datatype Addr = Addr(blkno: Blkno, off: nat)
+    type Object = seq<byte>
 
-function method objSize(obj: Object): nat
-{
-    |obj| * 8
-}
-
-function method zeroObject(k: Kind): (obj:Object)
-requires k >= 3
-ensures objSize(obj) == kindSize(k)
-{
-    kind_at_least_byte(k);
-    repeat(0 as bv8, kindSize(k)/8)
-}
-
-function method addrsForKinds(kinds: map<Blkno, Kind>): (addrs:set<Addr>)
-ensures forall a:Addr :: (&& a.blkno in kinds
-                          && 0 <= a.off < 4096*8
-                          && a.off % kindSize(kinds[a.blkno]) == 0) <==> a in addrs
-{
-    var addrs := set blkno : Blkno, off : int |
-    && blkno in kinds
-    && 0 <= off < 4096*8
-    :: Addr(blkno, off);
-    assert forall a:Addr :: a.blkno in kinds && 0 <= a.off < 4096*8 ==> a in addrs;
-    // NOTE: need to create the set above and then restrict it for Dafny's
-    // finite set comprehension heuristics to work
-    set a:Addr |
-    && a in addrs
-    && (var k := kinds[a.blkno];
-        a.off % kindSize(k) == 0)
-}
-
-class Jrnl
-{
-    var data: map<Addr, Object>;
-    // we cache the domain of data to easily show that it's constant
-    // NOTE: the entire Jrnl object is a spec, so having ghost state in it is
-    // really strange (it's state that isn't even needed to specify the object's
-    // behavior)
-    ghost const domain: set<Addr>;
-    const kinds: map<Blkno, Kind>;
-
-    predicate Valid()
-    reads this
+    function method objSize(obj: Object): nat
     {
-        && (forall a :: a in data ==>
-            && a.blkno in kinds
-            && objSize(data[a]) == kindSize(kinds[a.blkno]))
-        && (forall a :: a in data <==> a in domain)
+        |obj| * 8
     }
 
-    constructor(kinds: map<Blkno, Kind>)
-    requires forall blkno | blkno in kinds :: blkno >= 513
-    requires forall blkno | blkno in kinds :: kinds[blkno] >= 3
-    ensures Valid()
-    ensures forall a:Addr :: (&& a.blkno in kinds
-                              && a.off < 4096*8
-                              && (var k := kinds[a.blkno];
-                                a.off % kindSize(k) == 0)) <==>
-                             a in domain
-    ensures this.kinds == kinds
-    ensures forall a:Addr :: a in domain ==>
-            data[a] == zeroObject(kinds[a.blkno])
+    function method zeroObject(k: Kind): (obj:Object)
+    requires k >= 3
+    ensures objSize(obj) == kindSize(k)
     {
-        this.kinds := kinds;
-        var data: map<Addr, Object> :=
-            map a:Addr | a in addrsForKinds(kinds)
-                         :: zeroObject(kinds[a.blkno]);
-        assert forall a:Addr :: a in data <==>
-             && a.blkno in kinds
-             && a.off < 4096*8
-             && a.off % kindSize(kinds[a.blkno]) == 0;
-        this.data := data;
-        this.domain := map_domain(data);
+        kind_at_least_byte(k);
+        repeat(0 as bv8, kindSize(k)/8)
     }
 
-    function size(a: Addr): nat
-    reads this
-    requires Valid()
-    requires a in domain
+    class Jrnl
     {
-        kindSize(this.kinds[a.blkno])
-    }
+        var data: map<Addr, Object>;
+        // we cache the domain of data to easily show that it's constant
+        // NOTE: the entire Jrnl object is a spec, so having ghost state in it is
+        // really strange (it's state that isn't even needed to specify the object's
+        // behavior)
+        ghost const domain: set<Addr>;
+        ghost const kinds: map<Blkno, Kind>;
 
-    predicate has_kind(a: Addr, k: Kind)
-    reads this
-    requires Valid()
-    {
-        && a in domain
-        && kinds[a.blkno] == k
-    }
+        predicate Valid()
+        reads this
+        {
+            && (forall a :: a in data ==>
+                && a.blkno in kinds
+                && objSize(data[a]) == kindSize(kinds[a.blkno]))
+            && (forall a :: a in data <==> a in domain)
+        }
 
-    method Read(a: Addr, sz: nat)
-    returns (buf:Bytes)
-    requires Valid() ensures Valid()
-    requires a in domain && sz == size(a)
-    ensures
-    && fresh(buf)
-    && buf.Valid()
-    && buf.data == data[a]
-    && objSize(buf.data) == sz
-    {
-        ghost var k := kinds[a.blkno];
-        kindSize_bounds(k);
-        return new Bytes(data[a]);
-    }
+        constructor(kinds: map<Blkno, Kind>)
+        requires forall blkno | blkno in kinds :: blkno >= 513
+        requires forall blkno | blkno in kinds :: kinds[blkno] >= 3
+        ensures Valid()
+        ensures forall a:Addr :: (&& a.blkno in kinds
+                                && a.off < 4096*8
+                                && (var k := kinds[a.blkno];
+                                    a.off % kindSize(k) == 0)) <==>
+                                a in domain
+        ensures this.kinds == kinds
+        ensures forall a:Addr :: a in domain ==>
+                && data[a] == zeroObject(kinds[a.blkno])
 
-    method Write(a: Addr, bs: Bytes)
-    modifies this
-    requires Valid() ensures Valid()
-    requires bs.Valid()
-    requires a in domain && objSize(bs.data) == size(a)
-    ensures data == old(data)[a:=bs.data]
-    {
-        data := data[a:=bs.data];
+
+        function size(a: Addr): nat
+        reads this
+        requires Valid()
+        requires a in domain
+        {
+            kindSize(this.kinds[a.blkno])
+        }
+
+        predicate has_kind(a: Addr, k: Kind)
+        reads this
+        requires Valid()
+        {
+            && a in domain
+            && kinds[a.blkno] == k
+        }
+
+        method {:extern} Read(a: Addr, sz: nat)
+        returns (buf:Bytes)
+        requires Valid() ensures Valid()
+        requires a in domain && sz == size(a)
+        ensures
+        && fresh(buf)
+        && buf.Valid()
+        && buf.data == data[a]
+        && objSize(buf.data) == sz
+
+        method {:extern} Write(a: Addr, bs: Bytes)
+        modifies this
+        requires Valid() ensures Valid()
+        requires bs.Valid()
+        requires a in domain && objSize(bs.data) == size(a)
+        ensures data == old(data)[a:=bs.data]
     }
-}
 
 }
