src/Dafny/jrnl/jrnl.model.dfy
@@ -1,0 +1,51 @@
+include "jrnl.s.dfy"
+include "../machine/machine.model.dfy"
+
+module Jrnl_model refines JrnlSpec {
+    function method addrsForKinds(kinds: map<Blkno, Kind>): (addrs:set<Addr>)
+    ensures forall a:Addr :: (&& a.blkno in kinds
+                            && 0 <= a.off < 4096*8
+                            && a.off % kindSize(kinds[a.blkno]) == 0) <==> a in addrs
+    {
+        var addrs := set blkno : Blkno, off : int |
+        && blkno in kinds
+        && 0 <= off < 4096*8
+        :: Addr(blkno, off);
+        assert forall a:Addr :: a.blkno in kinds && 0 <= a.off < 4096*8 ==> a in addrs;
+        // NOTE: need to create the set above and then restrict it for Dafny's
+        // finite set comprehension heuristics to work
+        set a:Addr |
+        && a in addrs
+        && (var k := kinds[a.blkno];
+            a.off % kindSize(k) == 0)
+    }
+
+    class Jrnl {
+        constructor(kinds: map<Blkno, Kind>)
+        {
+            var data: map<Addr, Object> :=
+                map a:Addr | a in addrsForKinds(kinds)
+                            :: zeroObject(kinds[a.blkno]);
+            assert forall a:Addr :: a in data <==>
+                && a.blkno in kinds
+                && a.off < 4096*8
+                && a.off % kindSize(kinds[a.blkno]) == 0;
+            this.kinds := kinds;
+            this.data := data;
+            this.domain := map_domain(data);
+        }
+
+        method Read(a: Addr, sz: nat)
+        returns (buf:Bytes)
+        {
+            ghost var k := kinds[a.blkno];
+            kindSize_bounds(k);
+            return new Bytes(data[a]);
+        }
+
+        method Write(a: Addr, bs: Bytes)
+        {
+            data := data[a:=bs.data];
+        }
+    }
+}
